src/compiler/core/OCL_compiler_floor1_examp.thy
@@ -594,74 +594,24 @@ definition "print_examp_def_st1 = (\<lambda> OclDefSt name l \<Rightarrow> boots
 definition "print_examp_def_st_defs = (\<lambda> _ \<Rightarrow> start_map Thy_lemmas_simp
   [ Lemmas_simps \<open>\<close> [ \<open>state.defs\<close>, \<open>const_ss\<close> ] ])"
 
-definition "merge_unique_gen f l = List.fold (List.fold (\<lambda>x. case f x of Some (x, v) \<Rightarrow> RBT.insert x v | None \<Rightarrow> id)) l RBT.empty"
-definition "merge_unique f l = RBT.entries (merge_unique_gen f l)"
-definition "merge_unique' f l = List_map (map_prod (\<lambda>s. \<lless>s\<ggreater>) id)
-                                        (merge_unique (map_option (map_prod String_to_list id) o f) l)"
-
-definition "print_pre_post_wff = (\<lambda> OclDefPP s_pre s_post \<Rightarrow> \<lambda> ocl.
- (\<lambda> l. (List_map Thy_lemma_by l, ocl))
-  (let a = \<lambda>f x. Expr_apply f [x]
-     ; b = \<lambda>s. Expr_basic [s]
-     ; d = hol_definition
-     ; l_st = D_state_rbt ocl in
-   case (List.assoc s_pre l_st, List.assoc s_post l_st) of (Some l_pre, Some l_post) \<Rightarrow>
-   [ Lemma_by
-      (flatten [\<open>basic_\<close>, s_pre, \<open>_\<close>, s_post, \<open>_wff\<close>])
-      [a \<open>WFF\<close> (Expr_pair (b s_pre) (b s_post))]
-      []
-      (Tacl_by [Tac_simp_add (List_map d (List_flatten
-        [ [ \<open>WFF\<close>, s_pre, s_post, const_oid_of \<open>\<AA>\<close> ]
-        , List_map
-            (\<lambda>(cpt, _). var_oid_uniq @@ natural_of_str (case cpt of Oid i \<Rightarrow> i))
-            (merge_unique ((\<lambda>x. Some (x, ())) o oidGetInh o fst) [l_pre, l_post])
-        , List_map fst (merge_unique' (\<lambda>(_, ocore). case ocore of OclDefCoreBinding (_, ocli) \<Rightarrow> Some (print_examp_instance_name (\<lambda>s. s @@ isub_of_str (Inst_ty ocli)) (inst_name ocli), ())) [l_pre, l_post])
-        , List_map
-            (\<lambda>(s_ty, _). const_oid_of (datatype_name @@ isub_of_str s_ty))
-            (merge_unique' (\<lambda>(_, ocore). case ocore of OclDefCoreBinding (_, ocli) \<Rightarrow> Some (Inst_ty ocli, ())) [l_pre, l_post]) ]))]) ] ))"
-
-definition "print_pre_post_where = (\<lambda> OclDefPP s_pre s_post \<Rightarrow> \<lambda> ocl.
- (\<lambda> l. ((List_map Thy_lemma_by o List_flatten) l, ocl))
-  (let a = \<lambda>f x. Expr_apply f [x]
-     ; b = \<lambda>s. Expr_basic [s]
-     ; d = hol_definition
-     ; l_st = D_state_rbt ocl in
-   case (List.assoc s_pre l_st, List.assoc s_post l_st) of (Some l_pre, Some l_post) \<Rightarrow>
-   let f_name = \<lambda>(cpt, ocore). Some (oidGetInh cpt, ocore)
-     ; rbt_pre = merge_unique_gen f_name [l_pre]
-     ; rbt_post = merge_unique_gen f_name [l_post]
-     ; filter_ocore = \<lambda>x_pers_oid. case (RBT.lookup rbt_pre x_pers_oid, RBT.lookup rbt_post x_pers_oid) of
-             (Some ocore1, Some ocore2) \<Rightarrow> (\<open>OclIsMaintained\<close>, case (ocore1, ocore2) of (OclDefCoreBinding _, OclDefCoreBinding _) \<Rightarrow> [(ocore1, s_pre), (ocore2, s_post)]
-)
-           | (Some ocore, None) \<Rightarrow> (\<open>OclIsDeleted\<close>, [(ocore, s_pre)])
-           | (None, Some ocore) \<Rightarrow> (\<open>OclIsNew\<close>, [(ocore, s_post)])
-     ; rbt = RBT.union rbt_pre rbt_post
-     ; l_oid_of = keys (RBT.fold (\<lambda>_. \<lambda> OclDefCoreBinding (_, ocli) \<Rightarrow> insert (const_oid_of (datatype_name @@ isub_of_str (Inst_ty ocli))) ()) rbt RBT.empty) in
-   List_map
-     (\<lambda>x_pers_oid.
-       let (x_where, l_ocore) = filter_ocore x_pers_oid in
-       List_map (\<lambda>(ocore, name_st).
-         let (x_where, x_name, x_pers_expr) =
-           ( x_where
-           , case ocore of OclDefCoreBinding (name, ocli) \<Rightarrow>
-               let name =
-                 if D_design_analysis ocl = Gen_only_design then
-                   print_examp_def_st_inst_var_name ocli name_st
-                 else
-                   name in
-               (Some (name, print_examp_instance_name (\<lambda>s. s @@ isub_of_str (Inst_ty ocli)) (inst_name ocli)), b name)) in
-         Lemma_by (flatten [var_oid_uniq, natural_of_str (case x_pers_oid of Oid i \<Rightarrow> i), s_pre, s_post, \<open>_\<close>, name_st, \<open>_\<close>, x_where])
-          [Expr_binop (Expr_pair (b s_pre) (b s_post)) \<open>\<Turnstile>\<close> (a x_where (x_pers_expr))]
-          []
-          (Tacl_by [Tac_simp_add (List_map d (List_flatten
-            [ case x_name of Some (x_pers, x_name) \<Rightarrow> [x_pers, x_name] | _ \<Rightarrow> []
-            , [ x_where, \<open>OclValid\<close>, s_pre, s_post, const_oid_of \<open>option\<close> ]
-            , List_map
-                (\<lambda>(cpt, _). var_oid_uniq @@ natural_of_str (case cpt of Oid i \<Rightarrow> i))
-                (merge_unique ((\<lambda>x. Some (x, ())) o oidGetInh o fst) [l_pre, l_post])
-            , l_oid_of ]))])) l_ocore)
-     (filter (\<lambda>x_pers_oid. list_ex (\<lambda> (OclDefCoreBinding _, _) \<Rightarrow> True)
-       (snd (filter_ocore x_pers_oid)))
-       (RBT.keys rbt)) ))"
+definition "print_pre_post = (\<lambda> OclDefPP name s_pre s_post \<Rightarrow> bootstrap_floor
+  (\<lambda>f ocl. (List_flatten [f ocl], ocl))
+  (\<lambda>ocl.
+    let pref_name = case name of Some n \<Rightarrow> n
+                               | None \<Rightarrow> \<open>WFF_\<close> @@ nat_of_str (length (D_ocl_env ocl))
+      ; f_comp = \<lambda>None \<Rightarrow> id | Some (_, f) \<Rightarrow> f
+      ; f_conv = \<lambda>msg.
+          \<lambda> OclDefPPCoreAdd ocl_def_state \<Rightarrow>
+              let n = pref_name @@ msg in
+              (OclDefPPCoreBinding n, Cons (OclAstDefState Floor1 (OclDefSt n ocl_def_state)))
+          | s \<Rightarrow> (s, id) in
+    List_map
+      Isab_thy_ocl_deep_embed_ast
+      (let o_pre = Some (f_conv \<open>_pre\<close> s_pre)
+         ; o_post = map_option (f_conv \<open>_post\<close>) s_post in
+       (f_comp o_pre o f_comp o_post)
+         [ OclAstDefPrePost Floor2 (OclDefPP name
+                                             (case\<^sub>O\<^sub>C\<^sub>a\<^sub>m\<^sub>l o_pre of Some (n, _) \<Rightarrow> n)
+                                             (map_option fst o_post)) ])))"
 
 end
